Defining finite maps

convert/connected_components.py
@@ -64,27 +64,26 @@ def compute_components(neighborhoods):
 
     return (vertices, roots)
 
-def c_representation(name, vertices):
-    c = f'  c := λ v : fin {name}.vertex_size,\n    match v with\n'
+def c_representation(vertices):
+    c = f'  c := λ v : ℕ,\n    match v with\n'
     for v in vertices:
-        c += f'    | ⟨ {v.id}, _ ⟩ := {v.c}\n'
-    c += '    | ⟨ _ , cond ⟩ := 0\n    end,'
+        c += f'    | {v.id} := {v.c}\n'
+    c += '    | _ := 0\n    end,'
     return c
 
-def h_representation(name, vertices):
-    h = f'  h := λ v : fin {name}.vertex_size,\n    match v with\n'
+def h_representation(vertices):
+    h = f'  h := λ v : ℕ,\n    match v with\n'
     for v in vertices:
-        h += f'    | ⟨ {v.id}, _ ⟩ := {v.h}\n'
-    h += '    | ⟨ _ , cond ⟩ := 0\n    end,'
+        h += f'    | {v.id} := {v.h}\n'
+    h += '    | _ := 0\n    end,'
     return h
 
-def connect_edges_representation(name, vertices):
+def connect_edges_representation(vertices):
     n = len(vertices)
-    h = f'  connect_edges := λ u v : fin {name}.vertex_size,\n    match u, v with\n'
-    for i in range(n):
-        for j in range(n):
-            h += f'    | ⟨ {i}, _ ⟩, ⟨ {j}, _ ⟩ := begin intro _, bool_reflect end\n'
-    h += f'    | ⟨ _, _ ⟩, ⟨ _, _ ⟩ := sorry\n'
+    h = f'  connect_edges := \n'
+    h += f'    begin\n'
+    h += f'      apply tset.forall_is_forall,\n'
+    h += f'      bool_reflect\n'
     h += f'    end,'
     return h
 
@@ -92,75 +91,61 @@ def root_representation(roots):
     num_components = len(roots)
     root_rep = f'  root := λ i : fin {num_components},\n    match i with\n'
     for root in roots:
-        root_rep += f'    | ⟨ {root[0]}, _ ⟩ := ⟨ {root[1]}, by bool_reflect ⟩\n'
-    root_rep += f'    | _ := ⟨ 0, by bool_reflect ⟩\n    end,'
+        root_rep += f'    | ⟨ {root[0]}, _ ⟩ := {root[1]}\n'
+    root_rep += f'    | _ := 0\n    end,'
     return root_rep
 
 def is_root_representation(roots):
     num_components = len(roots)
-    root_rep = f'  is_root := λ i : fin {num_components},\n    match i with\n'
+    root_rep = f'  is_root := λ i,\n    match i with\n'
     for root in roots:
-        root_rep += f'    | ⟨ {root[0]}, _ ⟩ := ⟨ by bool_reflect, by bool_reflect ⟩\n'
-    root_rep += f'    | _ := ⟨ sorry, sorry ⟩\n    end,'
+        root_rep += f'    | ⟨ {root[0]}, _ ⟩ := by bool_reflect\n'
+    root_rep += f'    | _ := sorry\n    end,'
     return root_rep
 
-def uniqueness_of_roots_representation(name, vertices):
-    h = f'  uniqueness_of_roots := λ v : fin {name}.vertex_size,\n    match v with\n'
+def uniqueness_of_roots_representation(vertices):
+    h = f'  uniqueness_of_roots := λ v,\n    match v with\n'
     for v in vertices:
         if v.h == 0:
-            h += f'    | ⟨ {v.id}, _ ⟩ := by bool_reflect\n'
+            h += f'    | {v.id} := by bool_reflect\n'
         else:
-            h += f'    | ⟨ {v.id}, _ ⟩ := by contradiction\n'            
-    h += '    | ⟨ _ , cond ⟩ := sorry\n    end,'
-    return h
-
-def next_representation(name, vertices):
-    h = f'  next := λ v : fin {name}.vertex_size,\n    match v with\n'
-    for v in vertices:
-        if v.next:
-            h += f'    | ⟨ {v.id}, _ ⟩ := ⟨ {v.next.id}, by bool_reflect ⟩\n'
-    h += '    | ⟨ _ , cond ⟩ := ⟨ 0, by bool_reflect ⟩\n    end,'
-    return h
-
-def height_cond_representation(name, vertices):
-    h = f'  height_cond := λ v : fin {name}.vertex_size,\n    match v with\n'
-    for v in vertices:
-        if v.h == 0:
-            h += f'    | ⟨ {v.id}, cond ⟩ :=\n    begin\n      intro h,\n      by_contra,\n      have H : {name}_witness._match_1 ⟨{v.id}, cond⟩ = {v.id},\n      bool_reflect,\n      sorry\n    end\n'
-        else:
-            h += f'    | ⟨ {v.id}, cond ⟩ :=\n    begin\n      intro h,\n      split,\n      apply (to_bool_iff ({name}.edge (fin.mk {v.next.id} _) (fin.mk {v.id} _))).mp,\n      exact edge_{v.next.id}_{v.id},\n      bool_reflect\n    end\n'
+            h += f'    | {v.id} := by contradiction\n'            
     h += '    | _ := sorry\n    end,'
     return h
 
-def edge_lemma_representation(name, s, t):
-    l = f'lemma edge_{s}_{t} : @decidable.to_bool\n'
-    l += f'  ({name}.edge (fin.mk {s} (by bool_reflect)) (fin.mk {t} (by bool_reflect)))\n'
-    l += f'  ({name}.edge_decidable (fin.mk {s} (by bool_reflect)) (fin.mk {t} (by bool_reflect)))\n'
-    l += '  = tt := by refl'
-    return l
+def next_representation(vertices):
+    h = f'  next := λ v,\n    match v with\n'
+    for v in vertices:
+        if v.next:
+            h += f'    | {v.id} := {v.next.id}\n'
+    h += '    | _ := 0\n    end,'
+    return h
+
+def height_cond_representation(vertices):
+    h = f'  height_cond := λ v,\n    match v with\n'
+    for v in vertices:
+        if v.h == 0:
+            h += f'    | {v.id} :=\n      begin\n        have nh : ¬ 0 < 0 := irrefl 0,\n        contradiction,\n      end\n'
+        else:
+            h += f'    | {v.id} :=\n      begin\n        simp [edge_relation, decidable.lt_by_cases],\n        bool_reflect,\n      end\n'
+    h += '    | _ := sorry\n    end,'
+    return h
+
 
 def lean_representation(name, vertices, roots):
     representation = ''
-    for vertex in vertices:
-        if vertex.next:
-            representation += edge_lemma_representation(name, vertex.next.id, vertex.id) + '\n\n'
 
     representation += f'def {name}_witness : num_components_witness :=\n'
     representation += f'let H : {name}.vertex_size = {len(vertices)} := by bool_reflect in\n'
     representation += f'{{ G := {name},\n'
     representation += f'  num_components := {len(roots)},\n'
-    representation += c_representation(name, vertices) + '\n'
-    representation += h_representation(name, vertices) + '\n'
-    representation += connect_edges_representation(name, vertices) + '\n'
+    representation += c_representation(vertices) + '\n'
+    representation += h_representation(vertices) + '\n'
+    representation += connect_edges_representation(vertices) + '\n'
     representation += root_representation(roots) + '\n'
     representation += is_root_representation(roots) + '\n'
-    representation += uniqueness_of_roots_representation(name, vertices) + '\n'
-    representation += next_representation(name, vertices) + '\n'
-    representation += height_cond_representation(name, vertices) + '\n}'
+    representation += uniqueness_of_roots_representation(vertices) + '\n'
+    representation += next_representation(vertices) + '\n'
+    representation += height_cond_representation(vertices) + '\n}'
 
     return representation
-
-# nbhds = [(0, [4]), (1, [4]), (2,[3]), (3,[2,4]), (4,[0,1,3])]
-
-# vertices = compute_components(nbhds)
-# print(vertices)
